\fbox{\begin{minipage}[tc]{\linewidth-2\fboxsep}\ifthenelse{\boolean{doraggedright}}{\raggedright}{}
	\textbf{Lagrange-Fundamental-Polynom} \linebreak[3]
	Seien St체tzpunkte \mbox{$\left(x_i, f_i\right)$} \mbox{$i = 0,.. , n$} gegeben:\linebreak[3]
	Suche Polynome \mbox{$\ell_j \in \Pi_n, j = 0, .., n $} mit \linebreak[3]
	\mbox{$\ell_j(x_k) = \left\{
	\begin{array}{c}
		1 : j = k\\
		0 : j \neq k
	\end{array}\right.$}; \linebreak[3]
	\mbox{$\displaystyle P\left(f|x_0, .., x_n\right)(x) \stackrel{?!}{=} \sum_{j=0}^{n} f_j \cdot \ell_j(x)$}; \linebreak[3]
	\mbox{$
		\displaystyle
		\ell_j =  \prod_{\begin{smallmatrix}i=0\\i\neq j\end{smallmatrix}}^n \frac{x-x_i}{x_j-x_i}$}
\end{minipage}}\vspace{\myspace}
\fbox{\begin{minipage}[tc]{\linewidth-2\fboxsep}\ifthenelse{\boolean{doraggedright}}{\raggedright}{}
	\textbf{Newton-Basis}: \linebreak[3]
	$ \displaystyle P\left(f|x_0, .., x_n\right)(x) = \sum_{i=0}^{n}b_i \omega_i(x) = \sum_{i=0}^{n}b_i \prod_{p=0}^{j} \left( x - x_p\right)$ \linebreak[3]
	$ \displaystyle b_k = f_{[x_0, .., x_k]}$ \linebreak[3]
	$ \displaystyle f_{[x_r, .., x_s]} = \left(f_{[x_{r+1}, .., x_s]} - f_{[x_r, .., x_{s-1}]} \right) / \left(x_r - x_s\right)$ \linebreak[3]
	$ \displaystyle \omega_j(x) = \prod_{i=0}^{j} \left( x - x_i\right), \omega_0(x) = 1$
\end{minipage}}\vspace{\myspace}
\fbox{\begin{minipage}[tc]{\linewidth-2\fboxsep}\ifthenelse{\boolean{doraggedright}}{\raggedright}{}
	Algorithmus: \textbf{Horner-Schema}
	\begin{algorithmic}[1]
		\State $p = b_n$
		\For{$k = n-1, .., 1, 0$}
			\State $p = b_n + (x-x_k) \cdot p$
		\EndFor
	\end{algorithmic}
\end{minipage}}\vspace{\myspace}
\fbox{\begin{minipage}[tc]{\linewidth-2\fboxsep}\ifthenelse{\boolean{doraggedright}}{\raggedright}{}
	\textbf{Absch채tzung}; \linebreak[3]
	Satz: Seien $x_0, .., x_n$ Paarweise unterschiedliche St체tzstellen, 
	$ x_i \in [a,b] $ und $f \in C^{n+1}\left( [a, b] \right)$. \linebreak[3]
	Dann gilt f체r $x \in [a, b]$ \linebreak[3]
	$ \left\vert f\left( x \right) - P\left( f|x_0, .., x_n \right)(x) \right\rvert \leq  \left\lvert \omega_{n+1} \right\rvert \displaystyle \max_{z \in [a, b]} \frac{ \left\lvert f^{(n+1)}(z) \right\rvert}{ (n+1)! } $
\end{minipage}}\vspace{\myspace}
\fbox{\begin{minipage}[tc]{\linewidth-2\fboxsep}\ifthenelse{\boolean{doraggedright}}{\raggedright}{}
	\arraycolsep=1.9pt\def\arraystretch{1.5}
	\begin{equation*}
%	\begin{array}
		\centering
		\begin{tabular}{r|c|c|c|c|c|}
			\cline{2-6}
			& $0^\circ$ &            $30^\circ$ &            $45^\circ$ &            $60^\circ$ & $90^\circ$ \\ \hline
			\multicolumn{1}{|l|}{$\sin(\alpha)$} &	       0 &         $\frac{1}{2}$ & $\frac{1}{2}\sqrt{2}$ & $\frac{1}{2}\sqrt{3}$ &          1 \\ \hline
			\multicolumn{1}{|l|}{$\cos(\alpha)$} &         1 & $\frac{1}{2}\sqrt{3}$ & $\frac{1}{2}\sqrt{2}$ &         $\frac{1}{2}$ &          0 \\ \hline
			\multicolumn{1}{|l|}{$\tan(\alpha)$} &	       0 & $\frac{1}{3}\sqrt{3}$ &                     1 &           $\sqrt{3}$  &         -- \\ \hline
			\multicolumn{1}{|l|}{$\cot(\alpha)$} &	      -- &            $\sqrt{3}$ &                     1 & $\frac{1}{3}\sqrt{3}$ &          0 \\ \hline
		\end{tabular}
%	\end{array}
	\end{equation*}
\end{minipage}}

























































